refactor(pomset): move of_seq lemmas to Build module
* minor refactoring

theories/concur/pomset.v
@@ -60,6 +60,7 @@ Local Open Scope order_scope.
 Local Open Scope fset_scope.
 Local Open Scope quotient_scope.
 Local Open Scope ra_terms.
+Local Open Scope ident_scope.
 Local Open Scope lposet_scope.
 
 Declare Scope pomset_scope.
@@ -176,39 +177,25 @@ Proof.
 Qed.
 
 Definition of_seq ls := 
-  let fE  := [fset e | e in nfresh ident0 (size ls)] in 
+  let fE  := [fset e | e in nfresh \i0 (size ls)] in 
   let lab := fun e : fE => (nth bot ls (encode (val e))) in
   let ica := fun e1 e2 : fE => (encode (val e1)).+1 == encode (val e2) in
   @build fE lab ica.
 
-End Build.
-
-Module Export Theory.
-Section Theory.
-Context (E : identType) (L : eqType).
-Variable (bot : L).
-Implicit Types (p : lfspreposet E L bot) (ls : seq L).
-
-Open Scope ident_scope.
-
-Lemma of_seq_lab_defined ls :
-  bot \notin ls ->
+Lemma of_seq_lab_defined ls : bot \notin ls ->
   forall (e : [fset e | e in nfresh \i0 (size ls)]),
-  nth bot ls (@encode E (val e)) != bot.
+    nth bot ls (@encode E (val e)) != bot.
 Proof.
   move=> /negP nbl [/= ?]; rewrite ?inE /= in_nfresh encode0=> ?.
   apply/negP; move: nbl=> /[swap]/eqP<-; apply; apply/mem_nth; lia.
 Qed.
 
-Lemma of_seq_finsupp ls :
-  bot \notin ls ->
-  finsupp (of_seq E bot ls) = [fset e | e in nfresh \i0 (size ls)].
-Proof.
-  move/of_seq_lab_defined/build_finsupp; exact.
-Qed.
+Lemma of_seq_finsupp ls : bot \notin ls -> 
+  finsupp (of_seq ls) = [fset e | e in nfresh \i0 (size ls)].
+Proof. move/of_seq_lab_defined/build_finsupp; exact. Qed.
 
 Lemma of_seq_lab ls e : 
-  fs_lab (of_seq E bot ls) e = nth bot ls (encode e).
+  fs_lab (of_seq ls) e = nth bot ls (encode e).
 Proof.
   rewrite /of_seq build_lab /= /sub_lift.
   case: insubP=> /= [?? ->|] //.
@@ -218,26 +205,36 @@ Proof.
   by move=> ?; rewrite nth_default.
 Qed.
 
-Lemma of_seq_fs_ica ls e1 e2 : 
-  let n := size ls in
-  fs_ica (of_seq E bot ls) e1 e2 = 
-  [&& (encode e1).+1 == encode e2,
-   e1 \in nfresh ident0 (size ls) & 
-   e2 \in nfresh ident0 (size ls)].
+Lemma of_seq_fs_ica ls e1 e2 : bot \notin ls -> 
+  fs_ica (of_seq ls) e1 e2 = 
+    [&& (encode e1).+1 == encode e2
+      , e1 \in finsupp (of_seq ls)
+      & e2 \in finsupp (of_seq ls)
+    ].
 Proof.
-  rewrite /of_seq build_ica /sub_rel_lift /=.
-  do 2 (case: insubP=>[[??]|/negbTE] /[! inE]-> /=; last by case: (_ == _)).
-  move=>->->; by rewrite andbT.
+  move=> labD; rewrite !of_seq_finsupp /of_seq //. 
+  rewrite build_ica /sub_rel_lift /=.
+  (* TODO: make some lemma for `sub_rel_lift` to handle this *)
+  case: insubP=>[[e1' in1]|/negbTE] /[! inE]-> /=; rewrite ?andbF //.
+  case: insubP=>[[e2' in2]|/negbTE] /[! inE]-> /=; rewrite ?andbF //.
+  by move=> -> ->; rewrite andbT.
 Qed.
 
-Lemma of_seq_fin_ica ls : 
-  bot \notin ls ->
-  fin_ica (of_seq E bot ls) =2
-  [rel e1 e2 |(encode (val e1)).+1 == encode (val e2)].
+Lemma of_seq_fin_ica ls : bot \notin ls ->
+  fin_ica (of_seq ls) =2 [rel e1 e2 | (encode (val e1)).+1 == encode (val e2)].
 Proof.
-  move/of_seq_finsupp=> fE; case=> /= ? + [/= ?].
-  rewrite /fin_ica /sub_rel_down /= fE ?inE of_seq_fs_ica=>->->; lattice.
+  move=> labD; case=> /= ? + [/= ?].
+  rewrite /fin_ica /sub_rel_down /= ?inE of_seq_fs_ica //. 
+  by move=> -> ->; rewrite !andbT. 
 Qed.
+
+End Build.
+
+Module Export Theory.
+Section Theory.
+Context (E : identType) (L : eqType).
+Variable (bot : L).
+Implicit Types (p : lfspreposet E L bot) (ls : seq L).
 
 Lemma lab_definedP p : 
   reflect {in finsupp p, forall e, fs_lab p e != bot} (lab_defined p).
